Common.v
@@ -20,3 +20,30 @@ Ltac head_hnf expr := let expr' := eval hnf in expr in head expr'.
 Ltac evar1_aware_destruct_bool x :=
   instantiate (1 := if x then _ else _);
   destruct x.
+
+Ltac subst_body :=
+  repeat match goal with
+           | [ H := _ |- _ ] => subst H
+         end.
+
+(** Test if a tactic succeeds, but always roll-back the results *)
+Tactic Notation "test" tactic3(tac) :=
+  try (first [ tac | fail 2 tac "does not succeed" ]; fail tac "succeeds"; [](* test for [t] solved all goals *)).
+
+(** [not tac] is equivalent to [fail tac "succeeds"] if [tac] succeeds, and is equivalent to [idtac] if [tac] fails *)
+Tactic Notation "not" tactic3(tac) := try ((test tac); fail 1 tac "succeeds").
+
+(** [atomic x] is the same as [idtac] if [x] is a variable or hypothesis, but is [fail 0] if [x] has internal structure. *)
+Ltac atomic x :=
+  idtac;
+  match x with
+    | _ => is_evar x; fail 1 x "is not atomic (evar)"
+    | ?f _ => fail 1 x "is not atomic (application)"
+    | (fun _ => _) => fail 1 x "is not atomic (fun)"
+    | forall _, _ => fail 1 x "is not atomic (forall)"
+    | let x := _ in _ => fail 1 x "is not atomic (let in)"
+    | match _ with _ => _ end => fail 1 x "is not atomic (match)"
+    | _ => is_fix x; fail 1 x "is not atomic (fix)"
+    | context[?E] => (* catch-all *) (not constr_eq E x); fail 1 x "is not atomic (has subterm" E ")"
+    | _ => idtac
+  end.
