TrustedServerSyncBox.v
@@ -1,0 +1,518 @@
+(** * A box to mirror a server over untrusted channels using encryption while preventing timing side channels (part of TCB) *)
+Require Import Coq.Program.Basics Coq.Numbers.Natural.Peano.NPeano Coq.Lists.List.
+Require Import FunctionApp EncryptionInterface TrustedTickBox TrustedEncryptBox TrustedDecryptBox.
+Require Import Common.
+
+Local Open Scope list_scope.
+Local Open Scope program_scope.
+
+Set Implicit Arguments.
+
+(** ** Summary
+
+    We implement a box that presents the interface of a server storing
+    unencrypted data.  It handles "compare and set" and "get"
+    requests, and raises "compare and set failed locally (returns
+    current state)", "compare and set succeeded locally", and "remote
+    conflict (returns desired state, current state, and common
+    ancestor)", and "updated current state".  The "compare and set"
+    operation accepts keys of any type, which allows the client to
+    correlate "compare and set" requests with their responses.
+    Additionally, we provide read access to the current state of the
+    remote server, and an "are we fully synced?"  boolean.
+
+    We maintain the following internal state:
+    - [remoteStateE] - state we think the remote server has right now (encrypted)
+    - [remoteStateD] - state we think the remote server has right now (decrypted)
+    - [localStateD] - state we want the remote server to have (decrypted)
+
+    We implement the following straight-forward events:
+
+    Client Events:
+
+    - [ssbClientGetUpdate] - When the client requests an
+      update from the server, we request an update from our remote
+      server, hidden behind a tick box.
+
+    - [ssbClientGetRemoteState of getRemoteKeyT] - When the client
+      wants to know the state of the remote server, we return
+      [remoteStateD].
+
+    - [ssbClientAskIsFullySynced of fullySyncedKeyT] - When the client
+      wants to know if we are fully synced, we return [localStateD =
+      remoteStateD].
+
+    - [ssbClientCompareAndSet of (curD newD : rawDataT) (key :
+      clientCASKeyT)] - When the client requests a compare and set, we
+      set [localStateD] to [newD] iff it was previously [curD].  On
+      success, we raise [ssbCASLocalSuccess key], and on failure, we
+      raise [ssbCASLocalFailure key localStateD].  We then schedule a
+      server CAS.
+
+    Server Events:
+
+    - [ssbServerGotUpdate (newE : encryptedDataT)] - When the server
+      provides us with an update, we decrypt it to [newD].  If we
+      fail, we inform the client that the remote server got messed up.
+      If we succeed, and it is different from [localStateD], we set
+      [localStateD] and [remoteStateD] to [newD], and push an update
+      to the client.  In all cases, we set [remoteStateE] to [newE].
+
+    Timed events:
+
+    - When it's time to do a server CAS, we compute an encryption
+      [localStateE] of [localStateD].  We then tell the server that if
+      it's state is [remoteStateE], it should replace it with
+      [localStateE].
+
+      - On success, we set [remoteStateE] to [localStateE] and
+        [remoteStateD] to [localStateD] (values all taken at time of
+        encryption).
+
+      - On failure (current state is [remoteStateE']), we attempt to
+        decrypt to [remoteStateD'].
+
+        - On decryption succeess, we set [remoteStateE] to
+          [remoteStateE'], and [remoteStateD] to [remoteStateD'].  We
+          then alert the client that there was a remote conflict
+          between [remoteStateD] (taken at time of encryption) and
+          [remoteStateD'], when trying to update [remoteStateD] to
+          [localStateD] (both taken at time of encryption).
+
+        - On decryption failure, set [remoteStateE] to
+          [remoteStateE'], clear [remoteStateD], and inform the client
+          that the remote server got messed up.
+
+  *)
+
+Module TrustedServerSyncBox (DataTypes : EncryptionDataTypes) (Algorithm : EncryptionAlgorithm DataTypes).
+  Import DataTypes.
+
+  Module Import TEB := TrustedEncryptBox DataTypes Algorithm.
+  Module Import TDB := TrustedDecryptBox DataTypes Algorithm.
+
+  Section trustedServerSyncBox.
+    Variables getRemoteKeyT fullySyncedKeyT clientCASKeyT : Type.
+    Variable d_eqb : rawDataT -> rawDataT -> bool.
+
+    Record ServerSyncBoxPreState
+      := { localStateD : rawDataT;
+           remoteStateD : option rawDataT;
+           remoteStateE : option encryptedDataT }.
+
+    (** snapshot of state at time of encryption request *)
+    Let encryptDataTagT := ServerSyncBoxPreState.
+    Let pre_cas_state := encryptDataTagT.
+    (** (curE, newE) *)
+    Let cas_state := ((encryptedDataT * encryptedDataT) * pre_cas_state)%type.
+    Inductive ssbDecryptTagT :=
+    | ssbDTGotUpdate (dataE : encryptedDataT)
+    | ssbDTCASFailure (frozenState : ServerSyncBoxPreState) (remoteE : encryptedDataT)
+    | ssbDTCASSuccess (frozenState : ServerSyncBoxPreState) (remoteE : encryptedDataT).
+
+    Record ServerSyncBoxState :=
+      {
+        ssbState :> ServerSyncBoxPreState;
+        ssbGetUpdateState : TickBoxState unit;
+        ssbCASState : TickBoxState cas_state;
+        ssbEncryptState : EncryptBoxState;
+        ssbDecryptState : DecryptBoxState
+      }.
+
+(* python:
+<<
+fields=[(x.strip(), y.strip()) for x, y in [z.split(':') for z in """
+        ssbState : ServerSyncBoxPreState;
+        ssbGetUpdateState : TickBoxState unit;
+        ssbCASState : TickBoxState cas_state;
+        ssbEncryptState : EncryptBoxState;
+        ssbDecryptState : DecryptBoxState""".split(';')]]
+for field0, ty0 in fields:
+    body = ';\n          '.join((('%s := st.(%s)' % (field, field)) if field != field0 else ('%s := v' % field))
+                                for field, ty in fields)
+    print('  Definition set_%s (st : ServerSyncBoxState) (v : %s)' % (field0, ty0))
+    print('    := {| ' + body + ' |}.\n')
+>> *)
+
+  Definition set_ssbState (st : ServerSyncBoxState) (v : ServerSyncBoxPreState)
+    := {| ssbState := v;
+          ssbGetUpdateState := st.(ssbGetUpdateState);
+          ssbCASState := st.(ssbCASState);
+          ssbEncryptState := st.(ssbEncryptState);
+          ssbDecryptState := st.(ssbDecryptState) |}.
+
+  Definition set_ssbGetUpdateState (st : ServerSyncBoxState) (v : TickBoxState unit)
+    := {| ssbState := st.(ssbState);
+          ssbGetUpdateState := v;
+          ssbCASState := st.(ssbCASState);
+          ssbEncryptState := st.(ssbEncryptState);
+          ssbDecryptState := st.(ssbDecryptState) |}.
+
+  Definition set_ssbCASState (st : ServerSyncBoxState) (v : TickBoxState cas_state)
+    := {| ssbState := st.(ssbState);
+          ssbGetUpdateState := st.(ssbGetUpdateState);
+          ssbCASState := v;
+          ssbEncryptState := st.(ssbEncryptState);
+          ssbDecryptState := st.(ssbDecryptState) |}.
+
+  Definition set_ssbEncryptState (st : ServerSyncBoxState) (v : EncryptBoxState)
+    := {| ssbState := st.(ssbState);
+          ssbGetUpdateState := st.(ssbGetUpdateState);
+          ssbCASState := st.(ssbCASState);
+          ssbEncryptState := v;
+          ssbDecryptState := st.(ssbDecryptState) |}.
+
+  Definition set_ssbDecryptState (st : ServerSyncBoxState) (v : DecryptBoxState)
+    := {| ssbState := st.(ssbState);
+          ssbGetUpdateState := st.(ssbGetUpdateState);
+          ssbCASState := st.(ssbCASState);
+          ssbEncryptState := st.(ssbEncryptState);
+          ssbDecryptState := v |}.
+
+    Inductive ssbConfigInput :=
+    | ssbGetUpdateConfig (_ : tbConfigInput)
+    | ssbCASConfig (_ : tbConfigInput)
+    | ssbSetMasterKey (key : masterKeyT).
+
+    Inductive ssbEventInput :=
+    | ssbTick (addedTickCount : nat)
+    | ssbClientGetUpdate
+    | ssbClientGetRemoteState (key : getRemoteKeyT)
+    | ssbClientAskIsFullySynced (key : fullySyncedKeyT)
+    | ssbClientCompareAndSet (key : clientCASKeyT) (curD newD : rawDataT)
+    | ssbServerGotUpdate (newE : encryptedDataT)
+    | ssbServerCASFailure (key : pre_cas_state) (claimedCurE realCurE newE : encryptedDataT)
+    | ssbServerCASSuccess (key : pre_cas_state) (newE : encryptedDataT)
+    | ssbSystemRandomness (randomness : systemRandomnessT) (tag : rawDataT * encryptDataTagT).
+
+
+    Definition ssbInput := (ssbConfigInput + ssbEventInput)%type.
+
+    Inductive ssbWarningOutput :=
+    | ssbGetUpdateWarning (_ : tbWarningOutput unit)
+    | ssbCASWarning (_ : tbWarningOutput cas_state)
+    | ssbEncryptError (_ : ebErrorOutput)
+    | ssbDecryptError (_ : dbErrorOutput ssbDecryptTagT)
+    | ssbWarningInvalidTransition (ev : ssbInput) (st : ServerSyncBoxState)
+    | ssbErrorNoCASBeforeGetUpdate.
+
+    Inductive ssbEventOutput :=
+    | ssbClientGotUpdate (data : rawDataT)
+    | ssbClientGotRemoteState (key : getRemoteKeyT) (data : option rawDataT)
+    | ssbClientRespondIsFullySynced (key : fullySyncedKeyT) (_ : bool)
+    | ssbClientCASSuccess (key : clientCASKeyT) (newD : rawDataT)
+    | ssbClientCASFailure (key : clientCASKeyT) (claimedCurD realCurD newD : rawDataT)
+    | ssbClientRemoteConflict (localD remoteD : rawDataT) (ancestorD : option rawDataT)
+    | ssbClientRemoteUpdateSuccess (oldD newD : rawDataT)
+    | ssbServerGetUpdate
+    | ssbServerCAS (key : pre_cas_state) (curE newE : encryptedDataT)
+    | ssbRequestSystemRandomness (howMuch : systemRandomnessHintT) (tag : rawDataT * encryptDataTagT).
+
+  Definition ssbOutput := (ssbWarningOutput + ssbEventOutput)%type.
+
+  Variable initRawData : rawDataT.
+  Context (world : Type)
+          (handle : ssbOutput -> action world).
+
+  Definition initState : ServerSyncBoxState :=
+    {|
+      ssbState := {| localStateD := initRawData;
+                     remoteStateD := None;
+                     remoteStateE := None |};
+      ssbGetUpdateState := TrustedTickBox.initState _;
+      ssbCASState := TrustedTickBox.initState _;
+      ssbEncryptState := TEB.initState;
+      ssbDecryptState := TDB.initState
+    |}.
+
+  Local Ltac handle_eq_false' :=
+    idtac;
+    match goal with
+      | _ => progress subst_body
+      | _ => intro
+      | _ => progress simpl in *
+      | [ H : appcontext[match ?E with _ => _ end] |- _ ] => (atomic E; destruct E)
+      | [ H : Some _ = None |- _ ] => solve [ inversion H ]
+      | [ H : None = Some _ |- _ ] => solve [ inversion H ]
+      | [ H : inl _ = inr _ |- _ ] => solve [ inversion H ]
+      | [ H : inr _ = inl _ |- _ ] => solve [ inversion H ]
+      | [ H : _::_ = nil |- _ ] => solve [ inversion H ]
+      | [ H : appcontext[match ?E with _ => _ end] |- _ ] => (revert H; case_eq E; intros)
+      | [ H : (_, _) = (_, _) |- _ ] => inversion H; clear H
+      | [ H : inl _ = inl _ |- _ ] => inversion H; clear H
+      | [ H : inr _ = inr _ |- _ ] => inversion H; clear H
+      | [ H : Some _ = Some _ |- _ ] => inversion H; clear H
+      | [ H : _::_ = _::_ |- _ ] => inversion H; clear H
+    end.
+
+  Local Ltac handle_eq_false :=
+    match goal with
+      | [ |- _ -> False ] => idtac
+    end;
+    subst_body; clear; intro;
+    abstract (repeat handle_eq_false').
+
+  Definition handle_ssbGetUpdate'
+             (st : ServerSyncBoxState)
+  : tbOutput unit * TickBoxState unit -> list ssbOutput * ServerSyncBoxState.
+  Proof.
+    refine (fun i =>
+              (match fst i with
+                | inl warning
+                  => inl (ssbGetUpdateWarning warning)::nil
+                | inr tbRequestDataUpdate
+                  => let upd := tickBoxLoopPreBody
+                                  (st.(ssbGetUpdateState))
+                                  (inr (tbValueReady tt)) in
+                     match fst upd as u return u = fst upd -> _ with
+                       | nil => fun _ => nil
+                       | inl warning::nil => fun _ => inl (ssbGetUpdateWarning warning)::nil
+                       | _ => fun H => match (_ H) : False with end
+                     end eq_refl
+                | inr (tbPublishUpdate val)
+                  => inr ssbServerGetUpdate::nil
+               end,
+               set_ssbGetUpdateState st (snd i)));
+    handle_eq_false.
+  Defined.
+
+  Definition fold_handler {outT stT}
+             (get : ServerSyncBoxState -> stT)
+             (set : ServerSyncBoxState -> stT -> ServerSyncBoxState)
+             (handle : ServerSyncBoxState -> outT * stT -> list ssbOutput * ServerSyncBoxState)
+             (st : ServerSyncBoxState)
+  : list outT * stT -> list ssbOutput * ServerSyncBoxState
+    := fun outs_st =>
+         fold_left (fun ls_st out =>
+                      let ls'_st' := handle (snd ls_st) (out, get (snd ls_st)) in
+                      (fst ls_st ++ fst ls'_st', snd ls'_st'))
+                   (fst outs_st)
+                   (nil, set st (snd outs_st)).
+
+  Definition handle_ssbGetUpdate
+    := fold_handler ssbGetUpdateState set_ssbGetUpdateState handle_ssbGetUpdate'.
+
+  Definition handle_ssbEncrypt
+             (st : ServerSyncBoxState)
+  : option (ebOutput encryptDataTagT) * EncryptBoxState -> list ssbOutput * ServerSyncBoxState.
+  Proof.
+    refine (fun i =>
+              let st' := set_ssbEncryptState st (snd i) in
+              (match fst i with
+                 | Some (inl warning)
+                   => inl (ssbEncryptError warning)::nil
+                 | Some (inr (ebRequestSystemRandomness howMuch tag))
+                   => (inr (ssbRequestSystemRandomness howMuch tag))::nil
+                 | Some (inr (ebEncrypted newE frozenState))
+                   => match frozenState.(remoteStateE) with
+                        | Some curE
+                          => (inr (ssbServerCAS frozenState curE newE))::nil
+                        | None => (inl ssbErrorNoCASBeforeGetUpdate)::nil
+                      end
+                 | None => nil
+               end,
+               st')).
+  Defined.
+
+  Definition handle_ssbCAS'
+             (st : ServerSyncBoxState)
+  : tbOutput cas_state * TickBoxState cas_state -> list ssbOutput * ServerSyncBoxState.
+  Proof.
+    refine (fun i =>
+              let st' := set_ssbCASState st (snd i) in
+              match fst i with
+                | inl warning
+                  => (inl (ssbCASWarning warning)::nil, st')
+                | inr (tbPublishUpdate val)
+                  => (inr ssbServerGetUpdate::nil, st')
+
+                | inr tbRequestDataUpdate
+
+                  (** request an encryption of the current state, and
+                      snapshot the current state so we can decide what
+                      to do when we get back the encrypted value *)
+
+                  => let encResult := encryptBoxLoopPreBody
+                                        (st.(ssbEncryptState))
+                                        (ebEncrypt (st.(localStateD)) (st.(ssbState))) in
+                     handle_ssbEncrypt st' encResult
+              end).
+  Defined.
+
+  Definition handle_ssbCAS
+    := fold_handler ssbCASState set_ssbCASState handle_ssbCAS'.
+
+  Definition handle_ssbDecrypt
+             (st : ServerSyncBoxState)
+  : option (dbOutput ssbDecryptTagT) * DecryptBoxState -> list ssbOutput * ServerSyncBoxState.
+  Proof.
+    refine (fun i =>
+              let st' := set_ssbDecryptState st (snd i) in
+              match fst i with
+
+                | Some (inl warning)
+                  => (inl (ssbDecryptError warning)::nil,
+                      set_ssbState
+                        st'
+                        ({| localStateD := st'.(localStateD);
+                            remoteStateD := None;
+                            remoteStateE :=
+                              (match warning with
+                                 | dbErrorInvalidData dataE _
+                                   => Some dataE
+                                 | _ => None
+                               end) |}))
+
+                | Some (inr (dbDecrypted dataD (ssbDTGotUpdate dataE)))
+                  => ((if d_eqb dataD st.(localStateD)
+                       then nil
+                       else (inr (ssbClientGotUpdate dataD))::nil),
+                      set_ssbState st' {| localStateD := dataD;
+                                          remoteStateD := Some dataD;
+                                          remoteStateE := Some dataE |})
+
+                | Some (inr (dbDecrypted remoteD (ssbDTCASFailure frozenState dataE)))
+                  => ((inr (ssbClientRemoteConflict
+                              (frozenState.(localStateD)) (* local *)
+                              remoteD
+                              (frozenState.(remoteStateD)) (* ancestor *)))::nil,
+                      set_ssbState st' {| localStateD := remoteD;
+                                          remoteStateD := Some remoteD;
+                                          remoteStateE := Some dataE |})
+
+                | Some (inr (dbDecrypted remoteD (ssbDTCASSuccess frozenState dataE)))
+                  => ((inr (ssbClientRemoteUpdateSuccess
+                              (frozenState.(localStateD)) (* oldD *)
+                              remoteD (* newD *)))::nil,
+                      set_ssbState st' {| localStateD := remoteD;
+                                          remoteStateD := Some remoteD;
+                                          remoteStateE := Some dataE |})
+
+                | None => (nil, st')
+
+              end).
+  Defined.
+
+  Definition serverSyncBoxLoopPreBody
+             (st : ServerSyncBoxState)
+  : ssbInput -> list ssbOutput * ServerSyncBoxState.
+  Proof.
+    refine (fun i =>
+              match i with
+
+                | inl (ssbGetUpdateConfig i')
+                  => handle_ssbGetUpdate
+                       st
+                       (tickBoxLoopPreBody
+                          (st.(ssbGetUpdateState))
+                          (inl i'))
+
+                | inl (ssbCASConfig i')
+                  => handle_ssbCAS
+                       st
+                       (tickBoxLoopPreBody
+                          (st.(ssbCASState))
+                          (inl i'))
+
+                | inl (ssbSetMasterKey newKey)
+                  => let (ls0, st0) := handle_ssbEncrypt
+                                         st
+                                         (encryptBoxLoopPreBody
+                                            (st.(ssbEncryptState))
+                                            (ebSetMasterKey _ newKey)) in
+                     let (ls1, st1) := handle_ssbDecrypt
+                                         st
+                                         (decryptBoxLoopPreBody
+                                            (st.(ssbDecryptState))
+                                            (dbSetMasterKey _ newKey)) in
+                     (ls0 ++ ls1, st1)
+
+                | inr (ssbTick addedTickCount)
+                  => let (ls0, st0) := handle_ssbGetUpdate
+                                         st
+                                         (tickBoxLoopPreBody
+                                            (st.(ssbGetUpdateState))
+                                            (inr (tbTick _ addedTickCount))) in
+                     let (ls1, st1) := handle_ssbCAS
+                                         st0
+                                         (tickBoxLoopPreBody
+                                            (st0.(ssbCASState))
+                                            (inr (tbTick _ addedTickCount))) in
+                     (ls0 ++ ls1, st1)
+
+                | inr ssbClientGetUpdate
+                  => handle_ssbGetUpdate
+                       st
+                       (tickBoxLoopPreBody
+                          (st.(ssbGetUpdateState))
+                          (inr (tbNotifyChange _)))
+
+                | inr (ssbClientGetRemoteState key)
+                  => ((inr (ssbClientGotRemoteState key (st.(remoteStateD))))::nil, st)
+
+                | inr (ssbClientAskIsFullySynced key)
+                  => let b := match st.(remoteStateD) with
+                                | None => false
+                                | Some remoteStateD' => d_eqb st.(localStateD) remoteStateD'
+                              end in
+                     ((inr (ssbClientRespondIsFullySynced key b))::nil, st)
+
+                | inr (ssbClientCompareAndSet key curD newD)
+                  => if d_eqb st.(localStateD) curD
+                     then (let st' := set_ssbState
+                                        st
+                                        {| localStateD := newD;
+                                           remoteStateD := st.(remoteStateD);
+                                           remoteStateE := st.(remoteStateE) |} in
+                           let (ls0, st0) := handle_ssbCAS
+                                               st'
+                                               (tickBoxLoopPreBody
+                                                  (st'.(ssbCASState))
+                                                  (inr (tbNotifyChange _))) in
+                           ((inr (ssbClientCASSuccess key newD))::ls0, st0))
+                     else ((inr (ssbClientCASFailure key curD st.(localStateD) newD))::nil, st)
+
+                | inr (ssbServerGotUpdate dataE)
+                  => handle_ssbDecrypt
+                       st
+                       (decryptBoxLoopPreBody
+                          (st.(ssbDecryptState))
+                          (dbDecrypt dataE (ssbDTGotUpdate dataE)))
+
+                | inr (ssbServerCASFailure frozenState claimedCurE realCurE newE)
+                  => handle_ssbDecrypt
+                       st
+                       (decryptBoxLoopPreBody
+                          (st.(ssbDecryptState))
+                          (dbDecrypt realCurE (ssbDTCASFailure frozenState realCurE)))
+
+                | inr (ssbServerCASSuccess frozenState newE)
+                  => handle_ssbDecrypt
+                       st
+                       (decryptBoxLoopPreBody
+                          (st.(ssbDecryptState))
+                          (dbDecrypt newE (ssbDTCASSuccess frozenState newE)))
+
+                | inr (ssbSystemRandomness randomness tag)
+                  => handle_ssbEncrypt
+                       st
+                       (encryptBoxLoopPreBody
+                          (st.(ssbEncryptState))
+                          (ebSystemRandomness randomness tag))
+
+              end).
+  Defined.
+
+  Definition serverSyncBoxLoopBody {T}
+             (serverSyncBoxLoop : ServerSyncBoxState -> T)
+             (st : ServerSyncBoxState)
+  : ssbInput -> action world * T
+    := fun i => let outs := fst (serverSyncBoxLoopPreBody st i) in
+                (fold_left compose (map handle outs) id,
+                 serverSyncBoxLoop (snd (serverSyncBoxLoopPreBody st i))).
+
+  CoFixpoint serverSyncBoxLoop (st : ServerSyncBoxState) :=
+    Step (serverSyncBoxLoopBody serverSyncBoxLoop st).
+
+  Definition serverSyncBox : process _ _ := serverSyncBoxLoop initState.
+End trustedServerSyncBox.
